Revert changes of vec_permute functions in Lib.IntVector

code/gf128/Hacl.Spec.GF128.Lemmas.fsti
@@ -8,12 +8,12 @@ module S = Spec.GF128
 
 #set-options "--z3rlimit 30 --max_fuel 0 --max_ifuel 0"
 
-let elem = S.elem
+let elem = S.elem_le
 let zero : elem = zero
 let one : elem = one
 
-let ( +% ) (a b:elem) : elem = fadd #S.gf128 a b
-let ( *% ) (a b:elem) : elem = fmul_be #S.gf128 a b
+let ( +% ) (a b:elem) : elem = fadd #S.gf128_le a b
+let ( *% ) (a b:elem) : elem = S.fmul_le a b
 
 val add_identity: a:elem -> Lemma (zero +% a == a)
 
