code/gf128/Hacl.Spec.GF128.Vec.fst
@@ -24,7 +24,7 @@ let elem2 = lseq elem 2
 
 let elem4 = lseq elem 4
 let fadd4 (a:elem4) (b:elem4) : elem4 = map2 fadd a b
-let fmul4 (a:elem4) (b:elem4) : elem4 = map2 (fun x y -> reverse (fmul (reverse x) (reverse y))) a b
+let fmul4 (a:elem4) (b:elem4) : elem4 = map2 Scalar.fmul_le a b
 
 let load_elem4 (b:lbytes 64) : elem4 =
   let b1 = load_felem_be #gf128 (sub b 0 16) in
@@ -43,9 +43,9 @@ let normalize4 (pre:elem4) (acc:elem4) : elem =
   fadd (fadd (fadd a.[0] a.[1]) a.[2]) a.[3]
 
 let load_precompute_r (r:elem) : elem4 =
-  let r2 = reverse (reverse r `fmul` reverse r) in
-  let r3 = reverse (reverse r `fmul` reverse r2) in
-  let r4 =reverse (reverse r `fmul` reverse r3) in
+  let r2 = r `Scalar.fmul_le` r in
+  let r3 = r `Scalar.fmul_le` r2 in
+  let r4 =r `Scalar.fmul_le` r3 in
   create4 r4 r3 r2 r
 
 let gf128_update4_add_mul (pre:elem4) (b:lbytes 64) (acc:elem) : Tot elem =
